src/burrow/indexing.v
@@ -276,9 +276,9 @@ Admitted.
 Lemma forall_equiv_branch_all_total_in_refinement_domain roi branch lt idx
   : branch_all_total_in_refinement_domain roi branch lt idx
     <-> forall pl, node_all_total_in_refinement_domain roi (node_of_pl branch pl) lt (plend pl). Admitted.
-    
-Definition plsplit (ln: list nat) : PathLoc. Admitted.
-
   
 End Indexing.
+
+Definition plsplit (ln: list nat) : PathLoc. Admitted.
+
 
